In Simulator abstract theory, switched to having the simulator's port index as the only theory parameter. Also switched dummy adversary theorem to using version of invoke lemma for termination metrics for functionalities that does not restrict outgoing adversarial port indices, as this is not needed for this proof.

common/UCCore.ec
@@ -643,8 +643,8 @@ module MI = MakeInt.MI.
 (* Converting Hoare lemmas about invariants and termination metrics
    for functionalities into equiv lemmas
 
-   lemmas for invoke also restrict destination adversarial
-   port indices for adversarial messages *)
+   lemmas for invoke have two forms, one of them restricting
+   destination adversarial port indices for adversarial messages *)
 
 (* init lemma for use with any functionality, Fun, with an invariant
    for which we know the corresponding hoare lemma *)
@@ -665,19 +665,46 @@ conseq
 sim.
 qed.
 
-(* invoke lemma for use with any functionality, Fun, with an invariant and
-   termination metric for which we know the corresponding hoare lemma *)
-
 lemma invoke_term_metric_hoare_implies_equiv (Fun <: FUNC)
+      (invar : glob Fun -> bool, tm : glob Fun -> int, n : int) :
+  hoare
+  [Fun.invoke :
+   invar (glob Fun) /\ tm (glob Fun) = n ==>
+   invar (glob Fun) /\
+   (res <> None => tm (glob Fun) < n)] =>
+  equiv
+  [Fun.invoke ~ Fun.invoke :
+   ={m, glob Fun} /\ invar (glob Fun){1} /\
+   tm (glob Fun){1} = n ==>
+   ={res, glob Fun} /\ invar (glob Fun){1} /\
+   (res{1} <> None => tm (glob Fun){1} < n)].
+proof.
+move => invoke_hoare.
+conseq
+  (_ : ={m, glob Fun} ==> ={glob Fun, res})
+  (_ :
+   invar (glob Fun) /\ tm (glob Fun) = n ==>
+   invar (glob Fun) /\
+   (res <> None => tm (glob Fun) < n))
+  (_ : true ==> true) => //.
+sim.
+qed.
+
+(* invoke lemma for use with any functionality, Fun, with an invariant
+   and termination metric, including restricting adversarial port
+   indices of outgoing adversarial messages, for which we know the
+   corresponding hoare lemma *)
+
+lemma invoke_term_metric_adv_pis_hoare_implies_equiv (Fun <: FUNC)
       (invar : glob Fun -> bool, tm : glob Fun -> int,
-       n : int, advpis : int fset) :
+       n : int, adv_pis : int fset) :
   hoare
   [Fun.invoke :
    invar (glob Fun) /\ tm (glob Fun) = n ==>
    invar (glob Fun) /\
    (res <> None =>
     tm (glob Fun) < n /\
-    ((oget res).`1 = Adv => (oget res).`2.`2 \in advpis))] =>
+    ((oget res).`1 = Adv => (oget res).`2.`2 \in adv_pis))] =>
   equiv
   [Fun.invoke ~ Fun.invoke :
    ={m, glob Fun} /\ invar (glob Fun){1} /\
@@ -685,7 +712,7 @@ lemma invoke_term_metric_hoare_implies_equiv (Fun <: FUNC)
    ={res, glob Fun} /\ invar (glob Fun){1} /\
    (res{1} <> None =>
     tm (glob Fun){1} < n /\
-    ((oget res{1}).`1 = Adv => (oget res{1}).`2.`2 \in advpis))].
+    ((oget res{1}).`1 = Adv => (oget res{1}).`2.`2 \in adv_pis))].
 proof.
 move => invoke_hoare.
 conseq
@@ -695,7 +722,7 @@ conseq
    invar (glob Fun) /\
    (res <> None =>
     tm (glob Fun) < n /\
-    ((oget res).`1 = Adv => (oget res).`2.`2 \in advpis)))
+    ((oget res).`1 = Adv => (oget res).`2.`2 \in adv_pis)))
   (_ : true ==> true) => //.
 sim.
 qed.
@@ -781,22 +808,6 @@ op adv_pis_rf_info (rfi : rf_info) : int fset =
   else rangeset rfi.`rfi_adv_pi_begin
        (nth1_adv_pi_end_params rfi rfi.`rfi_num_params + 1).
 
-op adv_pis_rf_info_first (rfi : rf_info) : int =
-  rfi.`rfi_adv_pi_begin.
-
-op adv_pis_rf_info_last (rfi : rf_info) : int =
-  if rfi.`rfi_num_params = 0
-  then rfi.`rfi_adv_pi_main_end
-  else nth1_adv_pi_end_params rfi rfi.`rfi_num_params.
-
-lemma adv_pis_rf_info_rangeset (rfi : rf_info) :
-  adv_pis_rf_info rfi =
-  rangeset (adv_pis_rf_info_first rfi) (adv_pis_rf_info_last rfi + 1).
-proof.
-rewrite /adv_pis_rf_info /adv_pis_rf_info_first /adv_pis_rf_info_last.
-by case (rfi.`rfi_num_params = 0).
-qed.
-
 op rf_info_valid (rfi : rf_info) : bool =
   1 <= rfi.`rfi_num_parties /\
   0 <= rfi.`rfi_num_subfuns /\
@@ -865,6 +876,22 @@ have /# :
   ! (nth1_adv_pi_begin_params rfi 1 <= i <=
      nth1_adv_pi_end_params rfi j) by
     elim => [// | j ge0_j IH j_plus1_good_par /#].
+qed.
+
+op adv_pis_rf_info_first (rfi : rf_info) : int =
+  rfi.`rfi_adv_pi_begin.
+
+op adv_pis_rf_info_last (rfi : rf_info) : int =
+  if rfi.`rfi_num_params = 0
+  then rfi.`rfi_adv_pi_main_end
+  else nth1_adv_pi_end_params rfi rfi.`rfi_num_params.
+
+lemma adv_pis_rf_info_rangeset (rfi : rf_info) :
+  adv_pis_rf_info rfi =
+  rangeset (adv_pis_rf_info_first rfi) (adv_pis_rf_info_last rfi + 1).
+proof.
+rewrite /adv_pis_rf_info /adv_pis_rf_info_first /adv_pis_rf_info_last.
+by case (rfi.`rfi_num_params = 0).
 qed.
 
 lemma adv_pis_rf_info_first_ge1 (rfi : rf_info) :
@@ -1467,21 +1494,11 @@ abstract theory Simulator.
 
 (* begin theory parameters *)
 
-op adv_pis_begin : int.  (* first adversarial port index of unit *)
-op adv_pis_end   : int.  (* last adversarial port index of unit *)
+(* adversarial port index of simulator *)
 
-axiom adv_pis_begin_ge1    : 1 <= adv_pis_begin.
-axiom adv_pis_begin_le_end : adv_pis_begin <= adv_pis_end.
+op sim_adv_pi : int.
 
-(* end theory parameters *)
-
-op sim_adv_pi : int      = adv_pis_begin.
-op adv_pis    : int fset = rangeset adv_pis_begin (adv_pis_end + 1).
-
-lemma sim_adv_pi_ge1 : 1 <= sim_adv_pi.
-proof.
-by rewrite /sim_adv_pi adv_pis_begin_ge1.
-qed.
+axiom sim_adv_pi_ge1 : 1 <= sim_adv_pi.
 
 (* end theory parameters *)
 
@@ -1824,11 +1841,12 @@ module (CombEnvAdv (Env : ENV, Adv : ADV) : ENV) (Inter : INTER) = {
 
 section.
 
-declare module Env       <: ENV{-MI, -CombEnvAdv}.
-declare module Adv       <: ADV{-MI, -CombEnvAdv, -Env}.
+declare module Env       <: ENV{-MI, -MS, -CombEnvAdv}.
+declare module Adv       <: ADV{-MI, -MS, -CombEnvAdv, -Env}.
 declare module RealFunc  <: FUNC{-MI, -CombEnvAdv, -Env, -Adv}.
-declare module IdealFunc <: FUNC{-MI, -CombEnvAdv, -Env, -Adv}.
-declare module SimCore   <: ADV{-MI, -CombEnvAdv, -Env, -Adv, -IdealFunc}.
+declare module IdealFunc <: FUNC{-MI, -MS, -CombEnvAdv, -Env, -Adv}.
+declare module SimCore   <:
+  ADV{-MI, -MS, -CombEnvAdv, -Env, -Adv, -IdealFunc}.
 
 declare op invar_rf : glob RealFunc -> bool.
 declare op term_rf  : glob RealFunc -> int.
@@ -1852,9 +1870,7 @@ declare axiom RealFunc_invoke (n : int) :
     ={m, glob RealFunc} /\ invar_rf (glob RealFunc){1} /\
     term_rf (glob RealFunc){1} = n ==>
     ={res, glob RealFunc} /\ invar_rf (glob RealFunc){1} /\
-    (res{1} <> None =>
-     term_rf (glob RealFunc){1} < n /\
-     ((oget res{1}).`1 = Adv => (oget res{1}).`2.`2 \in adv_pis))].
+    (res{1} <> None => term_rf (glob RealFunc){1} < n)].
 
 declare axiom ge0_term_if (gl : glob IdealFunc) :
   invar_if gl => 0 <= term_if gl.
@@ -1871,9 +1887,7 @@ declare axiom IdealFunc_invoke (n : int) :
     ={m, glob IdealFunc} /\ invar_if (glob IdealFunc){1} /\
     term_if (glob IdealFunc){1} = n ==>
     ={res, glob IdealFunc} /\ invar_if (glob IdealFunc){1} /\
-    (res{1} <> None =>
-     term_if (glob IdealFunc){1} < n /\
-     ((oget res{1}).`1 = Adv => (oget res{1}).`2.`2 \in adv_pis))].
+    (res{1} <> None => term_if (glob IdealFunc){1} < n)].
 
 declare axiom ge0_term_sc (gl : glob SimCore) :
   invar_sc gl => 0 <= term_sc gl.
@@ -1893,14 +1907,13 @@ declare axiom SimCore_invoke (n : int) :
     (res{1} <> None => term_sc (glob SimCore){1} < n)].
 
 local lemma bridge_real (func' : addr, in_guard' : int fset) &m :
+  exper_pre func' =>
   Pr[Exper(MI(RealFunc, Adv), Env).main(func', in_guard') @ &m : res] =
   Pr[Exper(MI(RealFunc, DummyAdv), CombEnvAdv(Env, Adv))
        .main(func', in_guard') @ &m : res].
 proof.
-byequiv => //.
-proc.
-inline*.
-sp; wp.
+move => ep_func'.
+byequiv => //; proc; inline*; sp; wp.
 seq 2 10 :
   (={glob RealFunc, glob Adv, glob Env} /\
    func{1} = func' /\ in_guard{1} = in_guard' /\
@@ -1928,16 +1941,45 @@ auto.
 qed.
 
 local lemma bridge_ideal (func' : addr, in_guard' : int fset) &m :
+  exper_pre func' => disjoint in_guard' (fset1 sim_adv_pi) =>
   Pr[Exper(MI(IdealFunc, MS(SimCore, Adv)), Env)
        .main(func', in_guard') @ &m : res] =
   Pr[Exper(MI(IdealFunc, MS(SimCore, DummyAdv)), CombEnvAdv(Env, Adv))
        .main(func', in_guard') @ &m : res].
 proof.
+move => ep_func' disj_ig'.
+byequiv => //; proc; inline*; sp; wp.
+seq 4 12 :
+  (={glob MS, glob IdealFunc, glob SimCore, glob Adv, glob Env} /\
+   func{1} = func' /\ in_guard{1} = in_guard' /\
+   func0{2} = func' /\ in_guard0{2} = in_guard' /\
+   MI.func{1} = func' /\ MI.in_guard{1} = in_guard' /\
+   MI.func{2} = func' /\ MI.in_guard{2} = in_guard' /\
+   CombEnvAdv.func{2} = func' /\ CombEnvAdv.in_guard{2} = in_guard' /\
+   MS.if_addr_opt{1} = None).
+swap{1} 1 1; swap{2} 8 4; swap{2} 3 8; swap{2} 1 9.
+call (_ : true).
+call (_ : true).
+call (_ : true).
+auto.
+call
+  (_ :
+   ={glob IdealFunc, glob SimCore, glob MS, glob Adv} /\
+   MI.func{1} = func' /\ MI.in_guard{1} = in_guard' /\
+   MI.func{2} = func' /\ MI.in_guard{2} = in_guard' /\
+   CombEnvAdv.func{2} = func' /\ CombEnvAdv.in_guard{2} = in_guard' /\
+   (MS.if_addr_opt{1} <> None => MS.if_addr_opt{1} = Some func')).
+proc.
+if => //.
+inline{1} 1; inline{2} 1; sp 3 4.
+rcondt{1} 1; first auto. rcondt{2} 1; first auto.
 admit.
+auto.
+auto.
 qed.
 
 lemma dummy_adv (func' : addr, in_guard' : int fset, b : real) &m :
-  exper_pre func' => disjoint in_guard' adv_pis =>
+  exper_pre func' => disjoint in_guard' (fset1 sim_adv_pi) =>
   `|Pr[Exper(MI(RealFunc, DummyAdv), CombEnvAdv(Env, Adv))
          .main(func', in_guard') @ &m : res] -
     Pr[Exper(MI(IdealFunc, MS(SimCore, DummyAdv)), CombEnvAdv(Env, Adv))
@@ -1947,16 +1989,17 @@ lemma dummy_adv (func' : addr, in_guard' : int fset, b : real) &m :
          .main(func', in_guard') @ &m : res]| <= b.
 proof.
 move => ep_func' disj_ig' reduct.
-by rewrite bridge_real bridge_ideal.
+by rewrite bridge_real // bridge_ideal.
 qed.
 
 end section.
 
 lemma dummy_adversary
-      (Env <: ENV{-MI, -CombEnvAdv}) (Adv <: ADV{-MI, -CombEnvAdv, -Env})
+      (Env <: ENV{-MI, -MS, -CombEnvAdv})
+      (Adv <: ADV{-MI, -MS, -CombEnvAdv, -Env})
       (RealFunc <: FUNC{-MI, -CombEnvAdv, -Env, -Adv})
-      (IdealFunc <: FUNC{-MI, -CombEnvAdv, -Env, -Adv})
-      (SimCore <: ADV{-MI, -CombEnvAdv, -Env, -Adv, -IdealFunc})
+      (IdealFunc <: FUNC{-MI, -MS, -CombEnvAdv, -Env, -Adv})
+      (SimCore <: ADV{-MI, -MS, -CombEnvAdv, -Env, -Adv, -IdealFunc})
       (invar_rf : glob RealFunc -> bool, term_rf : glob RealFunc -> int,
        invar_if : glob IdealFunc -> bool, term_if : glob IdealFunc -> int,
        invar_sc : glob SimCore -> bool, term_sc : glob SimCore -> int,
@@ -1968,9 +2011,7 @@ lemma dummy_adversary
    [RealFunc.invoke :
     invar_rf (glob RealFunc) /\ term_rf (glob RealFunc) = n ==>
     invar_rf (glob RealFunc) /\
-    (res <> None =>
-       term_rf (glob RealFunc) < n /\
-       ((oget res).`1 = Adv => (oget res).`2.`2 \in adv_pis))]) =>
+    (res <> None => term_rf (glob RealFunc) < n)]) =>
   (forall (gl : glob IdealFunc), invar_if gl => 0 <= term_if gl) =>
   hoare [IdealFunc.init : true ==> invar_if (glob IdealFunc)] =>
   (forall (n : int),
@@ -1978,9 +2019,7 @@ lemma dummy_adversary
    [IdealFunc.invoke :
     invar_if (glob IdealFunc) /\ term_if (glob IdealFunc) = n ==>
     invar_if (glob IdealFunc) /\
-    (res <> None =>
-       term_if (glob IdealFunc) < n /\
-       ((oget res).`1 = Adv => (oget res).`2.`2 \in adv_pis))]) =>
+    (res <> None => term_if (glob IdealFunc) < n)]) =>
   (forall (gl : glob SimCore), invar_sc gl => 0 <= term_sc gl) =>
   hoare [SimCore.init : true ==> invar_sc (glob SimCore)] =>
   (forall (n : int),
@@ -1989,7 +2028,7 @@ lemma dummy_adversary
     invar_sc (glob SimCore) /\ term_sc (glob SimCore) = n ==>
     invar_sc (glob SimCore) /\
     (res <> None => term_sc (glob SimCore) < n)]) =>
-  exper_pre func' => disjoint in_guard' adv_pis =>
+  exper_pre func' => disjoint in_guard' (fset1 sim_adv_pi) =>
   `|Pr[Exper(MI(RealFunc, DummyAdv), CombEnvAdv(Env, Adv))
          .main(func', in_guard') @ &m : res] -
     Pr[Exper(MI(IdealFunc, MS(SimCore, DummyAdv)), CombEnvAdv(Env, Adv))
